Get login XSRF verification working.
Since I had to add assumptions about who is a browser or a server in order
to prove the login XSRF property I wanted, use them to strengthen the
login safety property too.

Notable SVX2 framework changes:
- Enable BCT translation of SVX_Ops.Call, needed in the current
  implementation for nested messages when the outer message is trusted.
  To achieve this, move all SVX2 ops stuff to the SVX_Common assembly and
  use the new BCTOmitAttribute.  We could do the same for SVX1 if we want.
- Add ability to assume a party is a browser or a server or that a given
  message is sent only by browsers.  It was cleanest to specify these
  assumptions via API calls in the predicate, so do the same for ordinary
  trust assumptions and remove the trustedParties argument to Certify.
- Add "declarable predicates", an approach for participants to remember
  determinations they've made that avoids the soundness problems of
  stateful participant objects (which I hope to deprecate).

SVAuth/SVX2_Test_AuthorizationCodeFlow.cs
@@ -9,6 +9,10 @@ using Newtonsoft.Json;
 
 namespace SVAuth
 {
+    // Obviously, much of this is copy and paste from SVX2_Test_ImplicitFlow,
+    // but factoring out the commonality would have been a distraction from this
+    // exercise.  We'll see that factoring out when we migrate the real
+    // implementations to SVX2.
     public static class SVX2_Test_AuthorizationCodeFlow
     {
         static readonly Principal googlePrincipal = Principal.Of("Google");
@@ -105,6 +109,9 @@ namespace SVAuth
             public Principal SVXPrincipal => googlePrincipal;
             private GoogleAuthorizationCodeGenerator authorizationCodeGenerator = new GoogleAuthorizationCodeGenerator();
 
+            private DeclarablePredicate<Principal /*underlying client*/, string /*username*/> SignedInPredicate
+                = new DeclarablePredicate<Principal, string>();
+
             private Dictionary<Secret, AuthorizationCodeParams> authorizationCodeParamsDict = new Dictionary<Secret, AuthorizationCodeParams>();
 
             public string CodeEndpoint(PrincipalHandle client, string codeRequestStr)
@@ -116,7 +123,7 @@ namespace SVAuth
                     client);
 
                 // In reality, AuthenticateClient couldn't be done
-                // synchronously, so both TokenEndpoint and AuthenticateClient
+                // synchronously, so both CodeEndpoint and AuthenticateClient
                 // would be broken into a start and a callback.
                 var idpConc = AuthenticateClient(client);
 
@@ -144,9 +151,22 @@ namespace SVAuth
                 });
             }
 
+            // Write lambda by hand because all compiler-generated classes are
+            // currently excluded from decompilation of method bodies by CCI.
+            class SignedInDeclarer
+            {
+                internal Google_IdP outer;
+                internal IdPAuthenticationEntry entry;
+                internal void Declare()
+                {
+                    outer.SignedInPredicate.Declare(VProgram_API.UnderlyingPrincipal(entry.authenticatedClient), entry.googleUsername);
+                }
+            }
+
             public IdPAuthenticationEntry SVX_ConcludeClientAuthentication(IdPAuthenticationEntry entry)
             {
-                // TODO: Declare IdpSignedIn predicate here (or add to a dictionary).
+                var d = new SignedInDeclarer { outer = this, entry = entry };
+                SVX_Ops.Ghost(d.Declare);
                 VProgram_API.AssumeActsFor(entry.authenticatedClient, GoogleUserPrincipal(entry.googleUsername));
                 // Reuse the message... Should be able to get away with it.
                 return entry;
@@ -154,6 +174,11 @@ namespace SVAuth
 
             public AuthorizationCodeResponse SVX_MakeAuthorizationCodeResponse(AuthorizationCodeRequest req, IdPAuthenticationEntry idpConc)
             {
+                // In CodeEndpoint, we requested an IdPAuthenticationEntry for
+                // req.SVX_sender, but SVX doesn't know that, so we have to do a
+                // concrete check.
+                VProgram_API.Assert(req.SVX_sender == idpConc.authenticatedClient);
+
                 // With this expression inlined below, BCT silently mistranslated the code.
                 var theParams = new AuthorizationCodeParams
                 {
@@ -208,24 +233,29 @@ namespace SVAuth
                     googleUsername = theParams.googleUsername
                 };
             }
+
+            public bool Ghost_CheckSignedIn(Principal underlyingPrincipal, string username)
+            {
+                return SignedInPredicate.Check(underlyingPrincipal, username);
+            }
         }
 
         class StateParams
         {
-            internal string sessionId;
+            // We expect this to be a facet issued by the RP.
+            internal PrincipalHandle client;
         }
         class MattMerchant_Google_StateGenerator : SecretGenerator<StateParams>
         {
             protected override PrincipalHandle[] GetReaders(object theParams)
             {
                 var params2 = (StateParams)theParams;
-                return new PrincipalHandle[] { googlePrincipal, mattMerchantPrincipal,
-                    PrincipalFacet.Of(mattMerchantPrincipal, params2.sessionId) };
+                return new PrincipalHandle[] { googlePrincipal, mattMerchantPrincipal, params2.client };
             }
 
             protected override string RawGenerate(StateParams theParams)
             {
-                return "mattmerchant_google_state:" + theParams.sessionId;
+                return "mattmerchant_google_state:" + theParams.client;
             }
 
             protected override void RawVerify(StateParams theParams, string secretValue)
@@ -242,15 +272,16 @@ namespace SVAuth
 
             MattMerchant_Google_StateGenerator stateGenerator = new MattMerchant_Google_StateGenerator();
 
+            // Something here is tripping up BCT.  Just exclude it until we have
+            // fully as-needed translation.
+            [BCTOmitImplementation]
             public string LoginStart(PrincipalHandle client)
             {
                 var req = new AuthorizationCodeRequest
                 {
                     rpPrincipal = SVXPrincipal,
-                    // XXX This cast is a little contrived.  Decide if we want
-                    // to pass the client as a session ID or a facet or what.
                     state = stateGenerator.Generate(
-                        new StateParams { sessionId = ((PrincipalFacet)client).id },
+                        new StateParams { client = client },
                         SVXPrincipal)
                 };
                 authorizationCodeRequestStructure.Export(req, client, googlePrincipal);
@@ -283,13 +314,17 @@ namespace SVAuth
                 // validationResponse.googleUsername.
                 var conc = SVX_Ops.Call(SVX_SignInRP, authorizationCodeResponse, validationResponse);
 
-                SVX_Ops.Certify(conc, LoginSafety, new Principal[] { googlePrincipal, SVXPrincipal });
-                //SVX_Ops.Certify(conc, LoginXSRFPrevention, new Principal[] { });
+                SVX_Ops.Certify(conc, LoginSafety);
+                SVX_Ops.Certify(conc, LoginXSRFPrevention, Tuple.Create(googlePrincipal, typeof(Google_IdP)));
                 // AbandonAndCreateSession...
             }
 
             public ValidationRequest SVX_MakeValidationRequest(AuthorizationCodeResponse resp)
             {
+                // May as well fail fast.  It should also pass verification to do this in SVX_SignInRP.
+                // Pull new { ... } out to work around BCT mistranslation.
+                var stateParams = new StateParams { client = resp.SVX_sender };
+                stateGenerator.Verify(stateParams, resp.state);
                 return new ValidationRequest
                 {
                     authorizationCode = resp.authorizationCode,
@@ -308,39 +343,37 @@ namespace SVAuth
 
             public static bool LoginSafety(RPAuthenticationConclusion conc)
             {
-                var targets = new PrincipalHandle[3];
-                targets[0] = googlePrincipal;
-                targets[1] = mattMerchantPrincipal;
-                targets[2] = GoogleUserPrincipal(conc.googleUsername);
-                return VProgram_API.ActsForAny(conc.authenticatedClient, targets);
+                var googleUser = GoogleUserPrincipal(conc.googleUsername);
+                VProgram_API.AssumeTrustedServer(googlePrincipal);
+                VProgram_API.AssumeTrustedServer(mattMerchantPrincipal);
+                VProgram_API.AssumeTrusted(googleUser);
+
+                return VProgram_API.ActsFor(conc.authenticatedClient, googleUser);
             }
 
             public static bool LoginXSRFPrevention(RPAuthenticationConclusion conc)
             {
-                // TODO
-#if false
-                var targets = new PrincipalHandle[3];
-                targets[0] = googlePrincipal;
-                targets[1] = mattMerchantPrincipal;
-                targets[2] = GoogleUserPrincipal(conc.googleUsername);
-                return VProgram_API.ActsForAny(conc.authenticatedClient, targets);
-#endif
-                throw new NotImplementedException();
+                VProgram_API.AssumeTrustedServer(googlePrincipal);
+                VProgram_API.AssumeTrustedServer(mattMerchantPrincipal);
+                VProgram_API.AssumeTrustedBrowser(conc.authenticatedClient);
+
+                var idp = VProgram_API.GetParticipant<Google_IdP>(googlePrincipal);
+                return idp.Ghost_CheckSignedIn(VProgram_API.UnderlyingPrincipal(conc.authenticatedClient), conc.googleUsername);
             }
         }
 
         [BCTOmitImplementation]
-        static SVX2_Test_AuthorizationCodeFlow()
+        static void InitializeMessageStructures()
         {
             // In all cases, we only bother declaring the secret readers we
             // actually need for the protocol flow.  Maybe this is a bad habit.
 
-            authorizationCodeRequestStructure = new MessageStructure<AuthorizationCodeRequest>();
+            authorizationCodeRequestStructure = new MessageStructure<AuthorizationCodeRequest>() { BrowserOnly = true };
             authorizationCodeRequestStructure.AddSecret(nameof(AuthorizationCodeRequest.state),
                 // The sender (the client) gets implicitly added.
                 (msg) => new PrincipalHandle[] { msg.rpPrincipal });
 
-            authorizationCodeResponseStructure = new MessageStructure<AuthorizationCodeResponse>();
+            authorizationCodeResponseStructure = new MessageStructure<AuthorizationCodeResponse>() { BrowserOnly = true };
             authorizationCodeResponseStructure.AddSecret(nameof(AuthorizationCodeRequest.state),
                 (msg) => new PrincipalHandle[] { });
             authorizationCodeResponseStructure.AddSecret(nameof(AuthorizationCodeResponse.authorizationCode),
@@ -352,6 +385,12 @@ namespace SVAuth
 
             // Nothing interesting here.
             validationResponseStructure = new MessageStructure<ValidationResponse>();
+        }
+
+        // Do not BCTOmitImplementation this; it affects some static field initializers that we want.
+        static SVX2_Test_AuthorizationCodeFlow()
+        {
+            InitializeMessageStructures();
         }
 
         [BCTOmitImplementation]
