SVX_Common/SVX2/DeclarablePredicate.cs
@@ -1,0 +1,39 @@
+﻿using System;
+using System.Collections.Generic;
+using System.Diagnostics.Contracts;
+using System.Linq;
+using System.Threading.Tasks;
+
+namespace SVX2
+{
+    // Add as many as we need.
+    public class DeclarablePredicate<T1>
+    {
+        public void Declare(T1 arg1)
+        {
+            // It doesn't hurt to let people call this in non-ghost code if they
+            // are able to get all the arguments concretely.
+            if (VProgram_API.InVProgram)
+                Contract.Assume(Check(arg1));
+        }
+        [BCTOmitImplementation]
+        public bool Check(T1 arg1)
+        {
+            throw new NotImplementedException();
+        }
+    }
+
+    public class DeclarablePredicate<T1, T2>
+    {
+        public void Declare(T1 arg1, T2 arg2)
+        {
+            if (VProgram_API.InVProgram)
+                Contract.Assume(Check(arg1, arg2));
+        }
+        [BCTOmitImplementation]
+        public bool Check(T1 arg1, T2 arg2)
+        {
+            throw new NotImplementedException();
+        }
+    }
+}
